proving cmp_sufficient_lemma seems complicated

Powers.dfy
@@ -2,9 +2,11 @@ module Powers
 {
     function method {:opaque} power(b:int, e:nat) : int
         decreases e;
-        ensures b >= 0 ==> power(b, e) >= 0;
+        ensures b > 0 ==> power(b, e) > 0;
+        ensures b == 0 ==> power(b, e) == 0;
     {
-        if (e == 0) then 1
+        if b == 0 then 0
+        else if (e == 0) then 1
         else b * power(b, e - 1)
     }
 
